more on Steel effect (2 polymnadic binds, par, and frame)

ulib/experimental/Steel.Effect.fst
@@ -41,9 +41,12 @@ let ens_depends_only_on (#a:Type)
   (forall x h_pre (h_post:Mem.hheap (post x)) (h:Mem.heap{Mem.disjoint h_post h}).
      q h_pre x h_post <==> q h_pre x (Mem.join h_post h))
 
+type fp_prop (hp:Mem.hprop) =
+  q:(Mem.heap -> prop){q `Mem.depends_only_on_without_affinity` hp}
+
 type pre_t = Mem.hprop
 type post_t (a:Type) = a -> Mem.hprop
-type req_t (pre:pre_t) = q:(Mem.heap -> prop){q `Mem.depends_only_on_without_affinity` pre}
+type req_t (pre:pre_t) = fp_prop pre
 type ens_t (pre:pre_t) (a:Type) (post:post_t a) =
   q:(Mem.heap -> a -> Mem.heap -> prop){ens_depends_only_on q pre post}
 
@@ -66,8 +69,8 @@ type repr (a:Type) (pre:pre_t) (post:post_t a) (req:req_t pre) (ens:ens_t pre a 
   //   ens (Mem.heap_of_mem m0) x (Mem.heap_of_mem m1) /\
   //   preserves_frame pre (post x) m0 m1)
 
-let return (a:Type u#a) (x:a) (post:post_t a) (ens:ens_t (post x) a post)
-: repr a (post x) post (fun h -> ens h x h) ens
+let returnc (a:Type u#a) (x:a)
+: repr a Mem.emp (fun _ -> Mem.emp) (fun _ -> True) (fun _ r _ -> r == x)
 = fun _ -> x
 
 #push-options "--z3rlimit 50"
@@ -105,18 +108,64 @@ let if_then_else (a:Type) (pre:pre_t) (post:post_t a)
     (fun h -> (p ==> req_then h) /\ ((~ p) ==> req_else h))
     (fun h0 x h1 -> (p ==> ens_then h0 x h1) /\ ((~ p) ==> ens_else h0 x h1))
 
-reifiable reflectable
+reflectable
 layered_effect {
   Steel : a:Type -> pre:pre_t -> post:post_t a -> req:req_t pre -> ens:ens_t pre a post -> Effect
   with
   repr = repr;
-  return = return;
+  return = returnc;
   bind = bind;
   subcomp = subcomp;
   if_then_else = if_then_else
 }
 
-let par (#aL:Type) (#preL:pre_t) (#postL:post_t aL) (#lpreL:req_t preL) (#lpostL:ens_t preL aL postL)
+assume WP_monotonic_pure:
+  forall (a:Type) (wp:pure_wp a).
+    (forall (p q:pure_post a).
+       (forall x. p x ==> q x) ==>
+       (wp p ==> wp q))
+
+let bind_pure_steel (a:Type) (b:Type)
+  (wp:pure_wp a)
+  (pre_g:pre_t) (post_g:post_t b) (req_g:a -> req_t pre_g) (ens_g:a -> ens_t pre_g b post_g)
+  (f:unit -> PURE a wp) (g:(x:a -> repr b pre_g post_g (req_g x) (ens_g x)))
+: repr b pre_g post_g
+    (fun h -> wp (fun x -> req_g x h) /\ wp (fun _ -> True))
+    (fun h0 r h1 -> exists x. (~ (wp (fun r -> r =!= x))) /\ ens_g x h0 r h1)
+= fun m0 ->
+  let x = f () in
+  g x m0
+
+polymonadic_bind (PURE, Steel) |> Steel = bind_pure_steel
+
+unfold
+let polymonadic_bind_steel_pure_pre (#a:Type) (#b:Type)
+  (#pre_f:pre_t) (#post_f:Mem.hprop) (req_f:req_t pre_f) (ens_f:ens_t pre_f a (fun _ -> post_f))
+  (wp_g:a -> pure_wp b)
+: req_t pre_f
+= // assert (forall x (h0:Mem.hheap pre_f) h1 (h2:Mem.heap{Mem.disjoint h0 h2}).
+  //           ens_f h0 x h1 <==> ens_f (Mem.join h0 h2) x h1);
+  // assert (forall x h1 (h0:Mem.hheap pre_f) (h2:Mem.heap{Mem.disjoint h0 h2}).
+  //         (ens_f h0 x h1 ==> p) <==> (ens_f (Mem.join h0 h2) x h1 ==> p));
+  admit ();          
+  fun h -> req_f h /\ (forall x h1. ens_f h x h1 ==> (wp_g x) (fun _ -> True))
+
+let bind_steel_pure (a:Type) (b:Type)
+  (pre_f:pre_t) (post_f:Mem.hprop) (req_f:req_t pre_f) (ens_f:ens_t pre_f a (fun _ -> post_f))
+  (wp_g:a -> pure_wp b)
+  (f:repr a pre_f (fun _ -> post_f) req_f ens_f) (g:(x:a -> unit -> PURE b (wp_g x)))
+: repr b pre_f (fun _ -> post_f)
+    (polymonadic_bind_steel_pure_pre req_f ens_f wp_g)
+    (fun h0 r h1 -> exists x. ens_f h0 x h1 /\ (~ ((wp_g x) (fun y -> y =!= r))))
+= fun m0 ->
+  let x = f () in
+  g x ()
+
+
+polymonadic_bind (Steel, PURE) |> Steel = bind_steel_pure
+
+
+let par0 (#aL:Type) (#preL:pre_t) (#postL:post_t aL) (#lpreL:req_t preL) (#lpostL:ens_t preL aL postL)
   (f:repr aL preL postL lpreL lpostL)
   (#aR:Type) (#preR:pre_t) (#postR:post_t aR) (#lpreR:req_t preR) (#lpostR:ens_t preR aR postR)
   (g:repr aR preR postR lpreR lpostR)
@@ -127,27 +176,37 @@ let par (#aL:Type) (#preL:pre_t) (#postL:post_t aL) (#lpreL:req_t preL) (#lpostL
   (fun h0 (xL, xR) h1 -> lpreL h0 /\ lpreR h0 /\ lpostL h0 xL h1 /\ lpostR h0 xR h1)
 = Steel?.reflect (fun _ -> Sem.run #state 0 #_ #_ #_ #_ #_ (Sem.Par (Sem.Act f) (Sem.Act g)))
 
-#push-options "--admit_smt_queries true"  //the h0 =!= h1 part is not `depends_only_on`
-let lift_pure_steel (a:Type) (wp:pure_wp a) (p:Mem.hprop) (f:unit -> PURE a wp)
-: repr a p (fun _ -> p)
-  (fun _ -> wp (fun _ -> True) /\ True)
-  (fun h0 r h1 -> ~ (wp (fun x -> x =!= r \/ h0 =!= h1)))
-= admit ()
-#pop-options
+assume val par (#aL:Type) (#preL:pre_t) (#postL:post_t aL) (#lpreL:req_t preL) (#lpostL:ens_t preL aL postL)
+  (f:unit -> Steel aL preL postL lpreL lpostL)
+  (#aR:Type) (#preR:pre_t) (#postR:post_t aR) (#lpreR:req_t preR) (#lpostR:ens_t preR aR postR)
+  (g:unit -> Steel aR preR postR lpreR lpostR)
+: Steel (aL & aR)
+  (preL `Mem.star` preR)
+  (fun (xL, xR) -> postL xL `Mem.star` postR xR)
+  (fun h -> lpreL h /\ lpreR h)
+  (fun h0 (xL, xR) h1 -> lpreL h0 /\ lpreR h0 /\ lpostL h0 xL h1 /\ lpostR h0 xR h1)
 
-assume WP_monotonic_pure:
-  forall (a:Type) (wp:pure_wp a).
-    (forall (p q:pure_post a).
-       (forall x. p x ==> q x) ==>
-       (wp p ==> wp q))
 
-let bind_PURE_M (a:Type) (b:Type)
-  (wp:pure_wp a)
-  (pre_g:pre_t) (post_g:post_t b) (req_g:a -> req_t pre_g) (ens_g:a -> ens_t pre_g b post_g)
-  (f:unit -> PURE a wp) (g:(x:a -> repr b pre_g post_g (req_g x) (ens_g x)))
-: repr b pre_g post_g
-    (fun h -> wp (fun x -> req_g x h) /\ wp (fun _ -> True))
-    (fun h0 r h1 -> exists x. (~ (wp (fun r -> r =!= x))) /\ ens_g x h0 r h1)
-= fun m0 ->
-  let x = f () in
-  g x m0
+let frame0 (#a:Type) (#pre:pre_t) (#post:post_t a) (#req:req_t pre) (#ens:ens_t pre a post)
+  (f:repr a pre post req ens)
+  (frame:Mem.hprop)
+  (f_frame:fp_prop frame)
+: Steel a
+  (pre `Mem.star` frame)
+  (fun x -> post x `Mem.star` frame)
+  (fun h -> req h /\ f_frame h)
+  (fun h0 r h1 -> req h0 /\ ens h0 r h1 /\ f_frame h1)
+= Steel?.reflect (fun _ -> Sem.run #state 0 #_ #_ #_ #_ #_ (Sem.Frame (Sem.Act f) frame f_frame))
+
+
+assume val frame (#a:Type) (#pre:pre_t) (#post:post_t a) (#req:req_t pre) (#ens:ens_t pre a post)
+  (f:unit -> Steel a pre post req ens)
+  (frame:Mem.hprop)
+  (f_frame:fp_prop frame)
+: Steel a
+  (pre `Mem.star` frame)
+  (fun x -> post x `Mem.star` frame)
+  (fun h -> req h /\ f_frame h)
+  (fun h0 r h1 -> req h0 /\ ens h0 r h1 /\ f_frame h1)
+
+
